pumping lemma, ex5 and updates

Proofs/CFG.lean
@@ -66,6 +66,7 @@ inductive SigmaA : Type
 deriving Fintype, DecidableEq
 open SigmaA
 
+namespace Ga
 inductive NTA : Type
 | E | T | F
 deriving Fintype, DecidableEq
@@ -91,4 +92,186 @@ abbrev GA : CFG SigmaA :=
          (NTA.F, [lpar,E,rpar])}
    }
 
+end Ga
+
+namespace Gaa
+
+inductive NTAA : Type
+| E
+deriving Fintype, DecidableEq
+
+open NTAA
+open SigmaA
+open Sum
+
+abbrev GAA : CFG SigmaA :=
+{ NT := NTAA
+  S := E
+  P := { (E, [inl E,inr plus,inl E]),
+         (E, [inl E,inr times,inl E]),
+         (E, [inr a]),
+         (E, [inr lpar,inl E,inr rpar])}
+}
+
+end Gaa
 end CfgEx
+
+namespace ParseTrees
+
+open Lang
+open Cfg
+
+variable {Sigma : Type}[Alphabet Sigma]
+
+variable (G : CFG Sigma)
+
+open Sum
+
+mutual
+
+  inductive PT : G.NT → Type where
+  | node : ∀ {A} , ∀ {α} ,
+            (A , α ) ∈ G.P
+            → PTSent α → PT A
+
+  inductive PTSent : Sent G → Type where
+  | nil : PTSent []
+  | NT : ∀ {A α }, PT A → PTSent α → PTSent (inl A :: α)
+  | T : ∀ a {α} , PTSent α →  PTSent (inr a :: α)
+
+end
+
+mutual
+  def yield {A : G.NT} : PT G A → Word Sigma
+  | PT.node _ pα => yieldSent pα
+
+  def yieldSent {α : Sent G} : PTSent G α → Word Sigma
+  | PTSent.nil => []
+  | PTSent.NT pA pα  => yield pA ++ yieldSent pα
+  | PTSent.T a pα => a :: yieldSent pα
+
+end
+
+abbrev L_tree : Lang Sigma
+:= { w | ∃ p : PT G G.S , w = yield G p }
+
+theorem L_tree_ok : L_tree G = Cfg.L G := by sorry
+
+-- abbrev Amb : Prop
+-- := ∃ p p' : PT G G.S ,
+--           yield G p = yield G p'
+--           ∧ p ≠ p'
+
+abbrev Amb : Prop :=
+  ∃ (w : Word Sigma ) (A : G.NT) (t₁ t₂ : PT G A),
+    yield G t₁ = w ∧
+    yield G t₂ = w ∧
+    t₁ ≠ t₂
+
+end ParseTrees
+
+namespace ParseTreeEx
+
+open CfgEx.Gaa
+open ParseTrees
+open CfgEx
+open SigmaA
+open Sum
+
+abbrev p1 : PT GAA NTAA.E :=
+by
+  refine
+    PT.node (G := GAA) (A := NTAA.E) (α := [inl NTAA.E, inr plus, inl NTAA.E])
+      (by simp [GAA])
+      ?_
+  -- RHS: E plus E
+  refine
+    PTSent.NT (G := GAA)
+      (PT.node (G := GAA) (A := NTAA.E) (α := [inr a])
+        (by simp [GAA])
+        (PTSent.T (G := GAA) a (PTSent.nil (G := GAA))))
+      ?_
+  refine PTSent.T (G := GAA) plus ?_
+  refine
+    PTSent.NT (G := GAA)
+      (PT.node (G := GAA) (A := NTAA.E) (α := [inl NTAA.E, inr times, inl NTAA.E])
+        (by simp [GAA])
+        ?_)
+      (PTSent.nil (G := GAA))
+  -- RHS: E times E
+  refine
+    PTSent.NT (G := GAA)
+      (PT.node (G := GAA) (A := NTAA.E) (α := [inr a])
+        (by simp [GAA])
+        (PTSent.T (G := GAA) a (PTSent.nil (G := GAA))))
+      ?_
+  refine PTSent.T (G := GAA) times ?_
+  refine
+    PTSent.NT (G := GAA)
+      (PT.node (G := GAA) (A := NTAA.E) (α := [inr a])
+        (by simp [GAA])
+        (PTSent.T (G := GAA) a (PTSent.nil (G := GAA))))
+      (PTSent.nil (G := GAA))
+
+lemma p1_yield : yield GAA p1 = [a,plus,a,times,a] := by rfl
+
+abbrev p2 : PT GAA NTAA.E :=
+by
+  refine
+    PT.node (G := GAA) (A := NTAA.E) (α := [inl NTAA.E, inr times, inl NTAA.E])
+      (by simp [GAA])
+      ?_
+  -- RHS: E times E
+  refine
+    PTSent.NT (G := GAA)
+      (PT.node (G := GAA) (A := NTAA.E) (α := [inl NTAA.E, inr plus, inl NTAA.E])
+        (by simp [GAA])
+        ?_)
+      ?_
+  -- left: E plus E
+  refine
+    PTSent.NT (G := GAA)
+      (PT.node (G := GAA) (A := NTAA.E) (α := [inr a])
+        (by simp [GAA])
+        (PTSent.T (G := GAA) a (PTSent.nil (G := GAA))))
+      ?_
+  refine PTSent.T (G := GAA) plus ?_
+  refine
+    PTSent.NT (G := GAA)
+      (PT.node (G := GAA) (A := NTAA.E) (α := [inr a])
+        (by simp [GAA])
+        (PTSent.T (G := GAA) a (PTSent.nil (G := GAA))))
+      (PTSent.nil (G := GAA))
+  -- then `times` and the right `a`
+  refine PTSent.T (G := GAA) times ?_
+  refine
+    PTSent.NT (G := GAA)
+      (PT.node (G := GAA) (A := NTAA.E) (α := [inr a])
+        (by simp [GAA])
+        (PTSent.T (G := GAA) a (PTSent.nil (G := GAA))))
+      (PTSent.nil (G := GAA))
+
+lemma p2_yield : yield GAA p1 = [a,plus,a,times,a] := by rfl
+
+def rootOp : PT GAA NTAA.E → Option SigmaA
+| PT.node (A := _) (α := α) _ _ =>
+    match α with
+    | [Sum.inl _, Sum.inr op, Sum.inl _] => some op
+    | _ => none
+
+lemma p1p2 : (p1 : PT GAA NTAA.E) ≠ (p2 : PT GAA NTAA.E) := by
+  intro h
+  have : rootOp p1 = rootOp p2 := by
+    simp [h]
+  -- but the root operators differ:
+  -- `p1` is rooted at `plus`, `p2` is rooted at `times`.
+  -- So we get `some plus = some times`, contradiction.
+  simpa [p1, p2, rootOp, GAA] using this
+
+theorem amb_gaa : Amb GAA := by
+  refine ⟨[a,plus,a,times,a], NTAA.E, p1, p2, ?_, ?_, ?_⟩
+  . rfl
+  . rfl
+  . apply p1p2
+
+end ParseTreeEx
