Exercises/ex5.lean
@@ -1,0 +1,84 @@
+/-
+COMP2012 (LAC) 2026
+
+Exercise 5
+
+Construct a CFG and PDA for the language of bracket-matched
+words.
+
+Don't change anything else in this file!
+-/
+import Proofs.CFG
+import Mathlib.Tactic.DeriveFintype
+import Proofs.PDA
+
+namespace ex5
+
+open Lang Sum Cfg CFG Pda PDA
+
+/-
+Let SigmaPar be the alphabet of left and right brackets
+-/
+
+inductive SigmaPar : Type
+| lpar -- "⟨"
+| rpar -- "⟩"
+deriving Fintype, DecidableEq
+open SigmaPar
+
+/-
+We consider the language L : Lang Σ of bracket-matched words, words
+words in which every ⟨ is “closed” by a ⟩ occurring later in the word. For instance:
+• [] ∈ L -- ϵ ∈ L
+• [lpar,rpar] ∈ L -- ⟨⟩ ∈ L
+• [lpar,lpar,rpar,lpar,rpar,rpar] ∈ L -- ⟨⟩⟨⟩ ∈ L
+• [lpar,lpar,rpar] ∉ L   -- ⟨⟨⟩ ∉ L because it has more ⟨’s than ⟩’s,
+• [lpar,rpar,rpar] ∉ L   -- ⟨⟩⟩ ∉ L because it has more ⟩’s than ⟨’s,
+• [lpar,rpar,rpar,lpar] ∉ L -- ⟨⟩⟩⟨ ∉ L because the second ⟩ occurs before the corresponding ⟨.
+-/
+
+/- 1. Define a CFG for the language, you will also need to define an inductive type for the Non-terminals -/
+inductive NTPar : Type
+-- E.g. | NT1 | NT2 | ...
+deriving Fintype, DecidableEq
+open NTPar
+
+abbrev GPar : CFG SigmaPar
+:= { NT := sorry
+     S := sorry
+     P := sorry
+}
+
+/- 2. Define a PDA for the language -/
+-- You need to define inductive types for the states and the stack alphabet
+inductive QPar : Type
+-- E.g. | q0 | q1 | ...
+deriving Fintype, DecidableEq
+open QPar
+
+inductive ΓPar : Type
+-- E.g. | g0 | g1 | ...
+deriving Fintype, DecidableEq
+open ΓPar
+
+abbrev PPar : PDA SigmaPar
+:= { Q := sorry
+     Γ := sorry
+     s := sorry
+     Z₀ := sorry
+     F := sorry
+     δ q x z := sorry
+}
+
+-- 3. Show that ⟨⟩⟨⟩ ∈ L PPar
+-- you can either do this by spelling out the sequence of IDs in a comment or by proving
+theorem e3 : [SigmaPar.lpar,SigmaPar.lpar, SigmaPar.rpar,SigmaPar.lpar,SigmaPar.rpar, SigmaPar.rpar] ∈ L PPar := by
+     sorry
+-- in Lean.
+
+/-
+⟨⟩⟨⟩ ∈ L PPar because:
+(q0, lpar lpar rpar lpar rpar rpar, hash) ->
+...
+-/
+end ex5
