Lectures/L12.lean
@@ -1,0 +1,143 @@
+import Proofs.Lang
+open Lang
+
+variable (Sigma : Type)[Alphabet Sigma]
+
+open Sum
+
+structure CFG : Type 1 where
+  NT : Type
+  [alphNT : Alphabet NT]
+  S : NT
+  P : Finset (NT × Word (Sum NT Sigma))
+
+
+variable {Sigma : Type}[Alphabet Sigma]
+
+variable (G : CFG Sigma )
+
+abbrev Sent : Type -- Sentence Form
+:= Word (Sum G.NT Sigma)
+
+abbrev Deriv : Set (Sent G × Sent G)
+:= { (α , β) |
+      ∃ w w' : Sent G, ∃ A : G.NT, ∃ γ : Sent G,
+      α = w ++ [inl A] ++ w'
+      ∧ β = w ++ γ ++ w'
+      ∧ (A , γ) ∈ G.P
+}
+
+inductive DerivStar : Set (Sent G × Sent G)
+| refl : ∀ α , DerivStar (α,α)
+| step : ∀ α β γ,
+        Deriv G (α , β) → DerivStar (β, γ)
+         → DerivStar (α , γ)
+
+open Sum
+
+abbrev emb : Word Sigma → Sent G
+:= List.map inr
+
+abbrev L : Lang Sigma
+:= { w | DerivStar G ([inl G.S],emb G w)}
+
+-- A for Arithmetic
+
+inductive SigmaA : Type
+| a | plus | times | lpar | rpar
+deriving Fintype, DecidableEq
+-- a , + , * , ( , )
+
+namespace Ga
+
+-- Fin 3
+inductive NTA : Type
+| E | T | F
+deriving Fintype, DecidableEq
+
+open SigmaA
+open NTA
+open CFG
+
+abbrev GA : CFG SigmaA
+:= { NT := NTA,
+     S := E,
+     P := { (E , [ inl T ]),
+            (E , [ inl E , inr plus, inl T]),
+            (T , [ inl F]),
+            (T , [ inl T, inr times, inl F]),
+            (F , [ inr a]),
+            (F , [ inr lpar , inl E, inr rpar])
+            }
+}
+
+/-
+E -> T | E + T
+T -> F | T * F
+F -> a | ( E )
+-/
+
+end Ga
+
+/-
+E -> E + E | E * E | a | ( E )
+-/
+
+open SigmaA
+
+abbrev GAA : CFG SigmaA
+:= {
+    NT := Fin 1
+    S := 0
+    P := { (0 , [inl 0,inr plus,inl 0 ]),
+           (0 , [inl 0,inr times,inl 0]),
+           (0 , [inr a]),
+           (0 , [inr lpar,inl 0,inr rpar])
+    }
+}
+
+theorem today : L Ga.GA = L GAA := by sorry
+
+--- What is parse tree?
+--- What does it mean that a grammar ambiguous ?
+--- there is more than parse tree for at least one word.
+
+variable (G : CFG Sigma)
+
+mutual
+
+  inductive PT : G.NT → Type
+
+    | node : ∀ {A} , ∀ {α} , (A , α ) ∈ G.P
+        → PTSent α → PT A
+
+  inductive PTSent : Sent G → Type
+
+    | nil  : PTSent []
+    | NT : ∀ {A}, ∀ {α} ,
+        PT A → PTSent α → PTSent ((inl A)::α)
+    | T : ∀ a {α} , PTSent α → PTSent (inr a :: α)
+
+end
+
+open PT
+open PTSent
+
+variable (G : CFG Sigma)
+
+mutual
+
+  def yield {A : G.NT }: PT G A → Word Sigma
+  | node _ t => yieldSent t
+
+  def yieldSent {α : Sent G} : PTSent G α → Word Sigma
+  | nil => []
+  | NT t ts => yield t ++ yieldSent ts
+  | T a ts => a :: yieldSent ts
+
+end
+
+abbrev Amb : Prop
+:= ∃ w : Word Sigma ,
+   ∃ A : G.NT , ∃ t t' : PT G A , yield G t = w ∧ yield G t' = w
+   ∧ t ≠ t'
