Lectures/L13.lean
@@ -1,0 +1,149 @@
+import Proofs.Lang
+import Mathlib.Tactic.DeriveFintype
+
+namespace pda
+
+open Lang Lang.Examples SigmaABC
+variable (Sigma : Type)[Alphabet Sigma]
+
+-- What have we seen so far?
+/-
+Chomsky Hierarchy
+Level 3: Regular languages
+A language that can be represented by:
+ - a DFA
+ - an NFA
+ - A regular expression
+
+Level 2: Context-free languages
+ - Context-free grammars
+ - Pushdown automata
+
+NFA/DFA: Automata with limited memory
+Pushdown automata: NFA + stack
+-/
+abbrev anbn : Lang SigmaABC
+:= { a^n ++ b^n | (n : ℕ) }
+
+structure PDA : Type 1 where
+  Q : Type -- states
+  [alphQ : Alphabet Q]
+  Γ : Type -- Stack alphabet
+  [alphΓ : Alphabet Γ]
+  s : Q -- initial state
+  z₀ : Γ -- initial stack state
+  F : Finset Q -- set of final states
+  δ : Q → Option Sigma → Γ → Finset (Q × List Γ) -- transition function
+
+open PDA
+variable {Sigma : Type}[Alphabet Sigma]
+variable (P : PDA Sigma)
+
+inductive Γ₀ : Type
+| hash | one -- a
+deriving Fintype,DecidableEq
+open Γ₀
+
+abbrev P₁ : PDA SigmaABC
+:= {
+  Q := Fin 3
+  Γ := Γ₀
+  s := 0
+  z₀ := Γ₀.hash -- #
+  F := { 2 }
+  δ q x γ :=
+    match q, x, γ with
+    | 0, some a, z => {(0, [one,z])}
+    | 0, some b, one => {(1, [])}
+    | 0, none, Γ₀.hash => {(2,[])}
+    | 1, some b, one => {(1,[])}
+    | 1, none, Γ₀.hash => {(2,[])}
+    | _,_,_ => {}
+}
+
+abbrev ID : Type := P.Q × Word Sigma × List P.Γ
+-- instantaneous description
+
+inductive Step : (ID P × ID P) → Prop
+| read : ∀ q q' α x w z y ,
+    (q' , α ) ∈ P.δ q (some x) z
+    → Step ((q, x::w, z::y), (q', w, α ++ y))
+| silent : ∀ q q' α w z y ,
+    (q', α) ∈ P.δ q none z
+    → Step ((q, w, z::y), (q', w, α ++ y))
+
+inductive Star {A : Type}(R : A × A → Prop) : A × A → Prop
+| refl : ∀ a, Star R (a, a)
+| step : ∀ a b c, R (a, b) → Star R (b, c) → Star R (a,c)
+-- This is the transitive, reflexive closure of a relation
+-- I.e., the relation you get when you allow 0 or multiple
+-- applications of R (steps in the process of an automaton,
+-- or derivations within a CFG).
+
+/-
+Explicitly, Star (Step P) is this:
+inductive StepStar : (ID P × ID P) → Prop
+| refl : ∀ a , StepStar (a , a)
+| step : ∀ a b c , Step P (a , b)
+      → StepStar (b , c) → StepStar (a , c)
+-/
+
+-- Acceptance by ending in a final state
+abbrev L : Lang Sigma
+:= { w | ∃ q' γ ,
+    Star (Step P) ((P.s,w,[P.z₀]),(q',[],γ))
+                  ∧ q' ∈ P.F }
+
+-- Acceptance by clearing the stack upon finishing the word
+abbrev L_empty : Lang Sigma
+ := { w | ∃ q' ,
+      Star (Step P) ((P.s,w,[P.z₀]),(q',[],[])) }
+
+-- These two ways of defining a language are equivalent in
+-- the sense that there exist ways to translate a PDA
+-- using L into one using L_empty while accepting the same
+-- language.
+
+-- We prove these examples by explicitly walking through the
+-- parsing process of the PDA.
+example : [a,a,b,b] ∈ L P₁ := by
+  simp
+  exists []
+  apply Star.step
+  apply Step.read
+  constructor
+  apply Star.step
+  apply Step.read
+  constructor
+  apply Star.step
+  apply Step.read
+  constructor
+  apply Star.step
+  apply Step.read
+  constructor
+  apply Star.step
+  apply Step.silent
+  constructor
+  apply Star.refl
+
+example : [a,a,b,b] ∈ L_empty P₁ := by
+  simp
+  exists 2
+  apply Star.step
+  apply Step.read
+  constructor
+  apply Star.step
+  apply Step.read
+  constructor
+  apply Star.step
+  apply Step.read
+  constructor
+  apply Star.step
+  apply Step.read
+  constructor
+  apply Star.step
+  apply Step.silent
+  constructor
+  apply Star.refl
+
+end pda
