Proofs/PDA.lean
@@ -1,0 +1,88 @@
+import Proofs.Lang
+
+namespace Pda
+open Lang
+
+variable (Sigma : Type)[Alphabet Sigma]
+
+structure PDA : Type 1 where
+  Q : Type -- states
+  [alphQ : Alphabet Q]
+  Γ : Type -- Stack alphabet
+  [alphΓ : Alphabet Γ]
+  s : Q    -- initial state
+  Z₀ : Γ    -- initial stack
+  F : Finset Q -- set of final states
+  δ : Q → Option Sigma → Γ → Finset (Q × List Γ)
+
+open PDA
+
+variable {Sigma : Type}[Alphabet Sigma]
+variable (P : PDA Sigma)
+
+abbrev ID : Type := P.Q × Word Sigma × List P.Γ
+-- Instantanous Description
+
+inductive Step : (ID P × ID P ) → Prop
+| read : ∀ q q' α x w z γ ,
+    (q' , α ) ∈ P.δ q (some x) z →
+       Step ((q , x :: w, z :: γ) , (q' , w , α ++ γ ) )
+| silent : ∀ q q' α w z γ ,
+    (q' , α ) ∈ P.δ q none z →
+       Step ((q , w , z :: γ) , (q' , w , α ++ γ ) )
+
+inductive Star {A : Type}(R : A × A → Prop)
+    : A × A → Prop
+| refl : ∀ a , Star R (a , a)
+| step : ∀ a b c , R (a , b)
+      → Star R (b , c) → Star R (a , c)
+-- transitive, reflexive closure
+
+abbrev L : Lang Sigma
+:= { w | ∃ q' γ ,
+    Star (Step P) ((P.s,w,[P.Z₀]),(q',[],γ))
+                  ∧ q' ∈ P.F }
+
+abbrev L_empty : Lang Sigma
+ := { w | ∃ q' ,
+      Star (Step P) ((P.s,w,[P.Z₀]),(q',[],[])) }
+
+abbrev isDet : Prop
+:=  ∀ q x z ,
+    Fintype.card (P.δ q (some x) z) + Fintype.card (P.δ q none z) ≤ 1
+
+
+end Pda
+
+namespace PdaEx
+
+open Pda
+open Lang
+open Examples
+
+inductive Γ₁ : Type
+| hash | one -- a
+deriving Fintype, DecidableEq
+open Γ₁
+
+open SigmaABC
+open Option
+
+abbrev P₁ : PDA SigmaABC
+:= { Q := Fin 3
+     Γ := Γ₁
+     s := 0
+     Z₀ := hash
+     F := { 2 }
+     δ q x γ :=
+       match q , x , γ with
+        | 0 , some a , z  =>
+            { ( 0 , [one , z ]) }
+        | 0 , some b , Γ₁.one    =>
+            { (1 , []) }
+        | 1 , some b , one => { ( 1 , [])}
+        | 1 , none , Γ₁.hash => { ( 2 , [] )}
+        | _ , _ , _ => {} }
+
+
+end PdaEx
